projects/lib/gmp_goal.v
@@ -1781,8 +1781,12 @@ forall (b_pre: Z) (n_pre: Z) (ap_pre: Z) (rp_pre: Z) (cap2: Z) (cap1: Z) (l2: (@
 .
 
 Definition mpn_add_1_safety_wit_2 := 
-forall (b_pre: Z) (n_pre: Z) (ap_pre: Z) (rp_pre: Z) (cap2: Z) (cap1: Z) (l2: (@list Z)) (val: Z) (l: (@list Z)) (b: Z) (l'': (@list Z)) (l': (@list Z)) (val2: Z) (val1: Z) (l_2: (@list Z)) (i: Z) ,
-  [| ((unsigned_last_nbits (((Znth i l_2 0) + b )) (32)) >= b) |] 
+forall (b_pre: Z) (n_pre: Z) (ap_pre: Z) (rp_pre: Z) (cap2: Z) (cap1: Z) (l2: (@list Z)) (val: Z) (l: (@list Z)) (b: Z) (l'': (@list Z)) (l': (@list Z)) (val2: Z) (val1: Z) (l_2: (@list Z)) (i: Z) (a: Z) (l''': (@list Z)) ,
+  [| (l'' = (cons (a) (l'''))) |] 
+  &&  [| (0 <= i) |] 
+  &&  [| (i < n_pre) |] 
+  &&  [| (n_pre <= cap2) |] 
+  &&  [| ((unsigned_last_nbits (((Znth i l_2 0) + b )) (32)) >= b) |] 
   &&  [| (i < n_pre) |] 
   &&  [| (0 <= i) |] 
   &&  [| (i <= n_pre) |] 
@@ -1803,12 +1807,12 @@ forall (b_pre: Z) (n_pre: Z) (ap_pre: Z) (rp_pre: Z) (cap2: Z) (cap1: Z) (l2: (@
   &&  [| (cap2 <= 100000000) |] 
   &&  [| (n_pre > 0) |] 
   &&  [| (n_pre <= cap1) |]
-  &&  (store_uint_array_rec rp_pre i cap2 (replace_Znth ((i - i )) ((unsigned_last_nbits (((Znth i l_2 0) + b )) (32))) (l'')) )
+  &&  (store_uint_array rp_pre (i + 1 ) (replace_Znth (i) ((unsigned_last_nbits (((Znth i l_2 0) + b )) (32))) ((app (l') ((cons (a) (nil)))))) )
+  **  ((( &( "i" ) )) # Int  |-> i)
+  **  (store_uint_array_rec rp_pre (i + 1 ) cap2 l''' )
   **  (store_uint_array ap_pre n_pre l_2 )
   **  ((( &( "r" ) )) # UInt  |-> (unsigned_last_nbits (((Znth i l_2 0) + b )) (32)))
-  **  ((( &( "i" ) )) # Int  |-> i)
   **  (store_undef_uint_array_rec ap_pre n_pre cap1 )
-  **  (store_uint_array rp_pre i l' )
   **  ((( &( "b" ) )) # UInt  |-> 0)
   **  ((( &( "n" ) )) # Int  |-> n_pre)
   **  ((( &( "ap" ) )) # Ptr  |-> ap_pre)
@@ -1819,8 +1823,12 @@ forall (b_pre: Z) (n_pre: Z) (ap_pre: Z) (rp_pre: Z) (cap2: Z) (cap1: Z) (l2: (@
 .
 
 Definition mpn_add_1_safety_wit_3 := 
-forall (b_pre: Z) (n_pre: Z) (ap_pre: Z) (rp_pre: Z) (cap2: Z) (cap1: Z) (l2: (@list Z)) (val: Z) (l: (@list Z)) (b: Z) (l'': (@list Z)) (l': (@list Z)) (val2: Z) (val1: Z) (l_2: (@list Z)) (i: Z) ,
-  [| ((unsigned_last_nbits (((Znth i l_2 0) + b )) (32)) < b) |] 
+forall (b_pre: Z) (n_pre: Z) (ap_pre: Z) (rp_pre: Z) (cap2: Z) (cap1: Z) (l2: (@list Z)) (val: Z) (l: (@list Z)) (b: Z) (l'': (@list Z)) (l': (@list Z)) (val2: Z) (val1: Z) (l_2: (@list Z)) (i: Z) (a: Z) (l''': (@list Z)) ,
+  [| (l'' = (cons (a) (l'''))) |] 
+  &&  [| (0 <= i) |] 
+  &&  [| (i < n_pre) |] 
+  &&  [| (n_pre <= cap2) |] 
+  &&  [| ((unsigned_last_nbits (((Znth i l_2 0) + b )) (32)) < b) |] 
   &&  [| (i < n_pre) |] 
   &&  [| (0 <= i) |] 
   &&  [| (i <= n_pre) |] 
@@ -1841,12 +1849,12 @@ forall (b_pre: Z) (n_pre: Z) (ap_pre: Z) (rp_pre: Z) (cap2: Z) (cap1: Z) (l2: (@
   &&  [| (cap2 <= 100000000) |] 
   &&  [| (n_pre > 0) |] 
   &&  [| (n_pre <= cap1) |]
-  &&  (store_uint_array_rec rp_pre i cap2 (replace_Znth ((i - i )) ((unsigned_last_nbits (((Znth i l_2 0) + b )) (32))) (l'')) )
+  &&  (store_uint_array rp_pre (i + 1 ) (replace_Znth (i) ((unsigned_last_nbits (((Znth i l_2 0) + b )) (32))) ((app (l') ((cons (a) (nil)))))) )
+  **  ((( &( "i" ) )) # Int  |-> i)
+  **  (store_uint_array_rec rp_pre (i + 1 ) cap2 l''' )
   **  (store_uint_array ap_pre n_pre l_2 )
   **  ((( &( "r" ) )) # UInt  |-> (unsigned_last_nbits (((Znth i l_2 0) + b )) (32)))
-  **  ((( &( "i" ) )) # Int  |-> i)
   **  (store_undef_uint_array_rec ap_pre n_pre cap1 )
-  **  (store_uint_array rp_pre i l' )
   **  ((( &( "b" ) )) # UInt  |-> 1)
   **  ((( &( "n" ) )) # Int  |-> n_pre)
   **  ((( &( "ap" ) )) # Ptr  |-> ap_pre)
@@ -1901,8 +1909,12 @@ forall (b_pre: Z) (n_pre: Z) (ap_pre: Z) (rp_pre: Z) (cap2: Z) (cap1: Z) (l2: (@
 .
 
 Definition mpn_add_1_entail_wit_2_1 := 
-forall (b_pre: Z) (n_pre: Z) (ap_pre: Z) (rp_pre: Z) (cap2: Z) (cap1: Z) (l2: (@list Z)) (val: Z) (l_2: (@list Z)) (b: Z) (l''_2: (@list Z)) (l'_2: (@list Z)) (val2_2: Z) (val1_2: Z) (l_3: (@list Z)) (i: Z) ,
-  [| ((unsigned_last_nbits (((Znth i l_3 0) + b )) (32)) < b) |] 
+forall (b_pre: Z) (n_pre: Z) (ap_pre: Z) (rp_pre: Z) (cap2: Z) (cap1: Z) (l2: (@list Z)) (val: Z) (l_2: (@list Z)) (b: Z) (l''_2: (@list Z)) (l'_2: (@list Z)) (val2_2: Z) (val1_2: Z) (l_3: (@list Z)) (i: Z) (a: Z) (l''': (@list Z)) ,
+  [| (l''_2 = (cons (a) (l'''))) |] 
+  &&  [| (0 <= i) |] 
+  &&  [| (i < n_pre) |] 
+  &&  [| (n_pre <= cap2) |] 
+  &&  [| ((unsigned_last_nbits (((Znth i l_3 0) + b )) (32)) < b) |] 
   &&  [| (i < n_pre) |] 
   &&  [| (0 <= i) |] 
   &&  [| (i <= n_pre) |] 
@@ -1923,10 +1935,10 @@ forall (b_pre: Z) (n_pre: Z) (ap_pre: Z) (rp_pre: Z) (cap2: Z) (cap1: Z) (l2: (@
   &&  [| (cap2 <= 100000000) |] 
   &&  [| (n_pre > 0) |] 
   &&  [| (n_pre <= cap1) |]
-  &&  (store_uint_array_rec rp_pre i cap2 (replace_Znth ((i - i )) ((unsigned_last_nbits (((Znth i l_3 0) + b )) (32))) (l''_2)) )
+  &&  (store_uint_array rp_pre (i + 1 ) (replace_Znth (i) ((unsigned_last_nbits (((Znth i l_3 0) + b )) (32))) ((app (l'_2) ((cons (a) (nil)))))) )
+  **  (store_uint_array_rec rp_pre (i + 1 ) cap2 l''' )
   **  (store_uint_array ap_pre n_pre l_3 )
   **  (store_undef_uint_array_rec ap_pre n_pre cap1 )
-  **  (store_uint_array rp_pre i l'_2 )
 |--
   EX (l'': (@list Z))  (l': (@list Z))  (val2: Z)  (val1: Z)  (l: (@list Z)) ,
   [| (0 <= (i + 1 )) |] 
@@ -1955,8 +1967,12 @@ forall (b_pre: Z) (n_pre: Z) (ap_pre: Z) (rp_pre: Z) (cap2: Z) (cap1: Z) (l2: (@
 .
 
 Definition mpn_add_1_entail_wit_2_2 := 
-forall (b_pre: Z) (n_pre: Z) (ap_pre: Z) (rp_pre: Z) (cap2: Z) (cap1: Z) (l2: (@list Z)) (val: Z) (l_2: (@list Z)) (b: Z) (l''_2: (@list Z)) (l'_2: (@list Z)) (val2_2: Z) (val1_2: Z) (l_3: (@list Z)) (i: Z) ,
-  [| ((unsigned_last_nbits (((Znth i l_3 0) + b )) (32)) >= b) |] 
+forall (b_pre: Z) (n_pre: Z) (ap_pre: Z) (rp_pre: Z) (cap2: Z) (cap1: Z) (l2: (@list Z)) (val: Z) (l_2: (@list Z)) (b: Z) (l''_2: (@list Z)) (l'_2: (@list Z)) (val2_2: Z) (val1_2: Z) (l_3: (@list Z)) (i: Z) (a: Z) (l''': (@list Z)) ,
+  [| (l''_2 = (cons (a) (l'''))) |] 
+  &&  [| (0 <= i) |] 
+  &&  [| (i < n_pre) |] 
+  &&  [| (n_pre <= cap2) |] 
+  &&  [| ((unsigned_last_nbits (((Znth i l_3 0) + b )) (32)) >= b) |] 
   &&  [| (i < n_pre) |] 
   &&  [| (0 <= i) |] 
   &&  [| (i <= n_pre) |] 
@@ -1977,10 +1993,10 @@ forall (b_pre: Z) (n_pre: Z) (ap_pre: Z) (rp_pre: Z) (cap2: Z) (cap1: Z) (l2: (@
   &&  [| (cap2 <= 100000000) |] 
   &&  [| (n_pre > 0) |] 
   &&  [| (n_pre <= cap1) |]
-  &&  (store_uint_array_rec rp_pre i cap2 (replace_Znth ((i - i )) ((unsigned_last_nbits (((Znth i l_3 0) + b )) (32))) (l''_2)) )
+  &&  (store_uint_array rp_pre (i + 1 ) (replace_Znth (i) ((unsigned_last_nbits (((Znth i l_3 0) + b )) (32))) ((app (l'_2) ((cons (a) (nil)))))) )
+  **  (store_uint_array_rec rp_pre (i + 1 ) cap2 l''' )
   **  (store_uint_array ap_pre n_pre l_3 )
   **  (store_undef_uint_array_rec ap_pre n_pre cap1 )
-  **  (store_uint_array rp_pre i l'_2 )
 |--
   EX (l'': (@list Z))  (l': (@list Z))  (val2: Z)  (val1: Z)  (l: (@list Z)) ,
   [| (0 <= (i + 1 )) |] 
@@ -2174,9 +2190,9 @@ forall (b_pre: Z) (n_pre: Z) (ap_pre: Z) (rp_pre: Z) (cap2: Z) (cap1: Z) (l2: (@
   **  (store_uint_array_rec rp_pre i cap2 l'' )
 .
 
-Definition mpn_add_1_partial_solve_wit_4 := 
+Definition mpn_add_1_partial_solve_wit_4_pure := 
 forall (b_pre: Z) (n_pre: Z) (ap_pre: Z) (rp_pre: Z) (cap2: Z) (cap1: Z) (l2: (@list Z)) (val: Z) (l: (@list Z)) (b: Z) (l'': (@list Z)) (l': (@list Z)) (val2: Z) (val1: Z) (l_2: (@list Z)) (i: Z) ,
-  [| ((unsigned_last_nbits (((Znth i l_2 0) + b )) (32)) < b) |] 
+  [| ((unsigned_last_nbits (((Znth i l_2 0) + b )) (32)) >= b) |] 
   &&  [| (i < n_pre) |] 
   &&  [| (0 <= i) |] 
   &&  [| (i <= n_pre) |] 
@@ -2198,39 +2214,22 @@ forall (b_pre: Z) (n_pre: Z) (ap_pre: Z) (rp_pre: Z) (cap2: Z) (cap1: Z) (l2: (@
   &&  [| (n_pre > 0) |] 
   &&  [| (n_pre <= cap1) |]
   &&  (store_uint_array ap_pre n_pre l_2 )
+  **  ((( &( "r" ) )) # UInt  |-> (unsigned_last_nbits (((Znth i l_2 0) + b )) (32)))
+  **  ((( &( "i" ) )) # Int  |-> i)
   **  (store_undef_uint_array_rec ap_pre n_pre cap1 )
   **  (store_uint_array rp_pre i l' )
   **  (store_uint_array_rec rp_pre i cap2 l'' )
+  **  ((( &( "b" ) )) # UInt  |-> 0)
+  **  ((( &( "n" ) )) # Int  |-> n_pre)
+  **  ((( &( "ap" ) )) # Ptr  |-> ap_pre)
+  **  ((( &( "rp" ) )) # Ptr  |-> rp_pre)
 |--
-  [| ((unsigned_last_nbits (((Znth i l_2 0) + b )) (32)) < b) |] 
+  [| (0 <= i) |] 
   &&  [| (i < n_pre) |] 
-  &&  [| (0 <= i) |] 
-  &&  [| (i <= n_pre) |] 
-  &&  [| (list_store_Z_compact l_2 val ) |] 
-  &&  [| (n_pre <= cap1) |] 
-  &&  [| (list_store_Z (sublist (0) (i) (l_2)) val1 ) |] 
-  &&  [| (list_store_Z l' val2 ) |] 
-  &&  [| ((val2 + (b * (Z.pow (UINT_MOD) (i)) ) ) = (val1 + b_pre )) |] 
-  &&  [| ((Zlength (l')) = i) |] 
-  &&  [| ((Zlength (l2)) = cap2) |] 
-  &&  [| (n_pre <= cap1) |] 
-  &&  [| ((Zlength (l)) = n_pre) |] 
-  &&  [| (cap1 <= 100000000) |] 
-  &&  [| (list_store_Z_compact l val ) |] 
-  &&  [| ((Zlength (l2)) = cap2) |] 
-  &&  [| (cap2 >= n_pre) |] 
-  &&  [| (cap1 <= 100000000) |] 
-  &&  [| (cap2 <= 100000000) |] 
-  &&  [| (n_pre > 0) |] 
-  &&  [| (n_pre <= cap1) |]
-  &&  (((rp_pre + (i * sizeof(UINT) ) )) # UInt  |->_)
-  **  (store_uint_array_missing_i_rec rp_pre i i cap2 l'' )
-  **  (store_uint_array ap_pre n_pre l_2 )
-  **  (store_undef_uint_array_rec ap_pre n_pre cap1 )
-  **  (store_uint_array rp_pre i l' )
+  &&  [| (n_pre <= cap2) |]
 .
 
-Definition mpn_add_1_partial_solve_wit_5 := 
+Definition mpn_add_1_partial_solve_wit_4_aux := 
 forall (b_pre: Z) (n_pre: Z) (ap_pre: Z) (rp_pre: Z) (cap2: Z) (cap1: Z) (l2: (@list Z)) (val: Z) (l: (@list Z)) (b: Z) (l'': (@list Z)) (l': (@list Z)) (val2: Z) (val1: Z) (l_2: (@list Z)) (i: Z) ,
   [| ((unsigned_last_nbits (((Znth i l_2 0) + b )) (32)) >= b) |] 
   &&  [| (i < n_pre) |] 
@@ -2258,7 +2257,174 @@ forall (b_pre: Z) (n_pre: Z) (ap_pre: Z) (rp_pre: Z) (cap2: Z) (cap1: Z) (l2: (@
   **  (store_uint_array rp_pre i l' )
   **  (store_uint_array_rec rp_pre i cap2 l'' )
 |--
-  [| ((unsigned_last_nbits (((Znth i l_2 0) + b )) (32)) >= b) |] 
+  [| (0 <= i) |] 
+  &&  [| (i < n_pre) |] 
+  &&  [| (n_pre <= cap2) |] 
+  &&  [| ((unsigned_last_nbits (((Znth i l_2 0) + b )) (32)) >= b) |] 
+  &&  [| (i < n_pre) |] 
+  &&  [| (0 <= i) |] 
+  &&  [| (i <= n_pre) |] 
+  &&  [| (list_store_Z_compact l_2 val ) |] 
+  &&  [| (n_pre <= cap1) |] 
+  &&  [| (list_store_Z (sublist (0) (i) (l_2)) val1 ) |] 
+  &&  [| (list_store_Z l' val2 ) |] 
+  &&  [| ((val2 + (b * (Z.pow (UINT_MOD) (i)) ) ) = (val1 + b_pre )) |] 
+  &&  [| ((Zlength (l')) = i) |] 
+  &&  [| ((Zlength (l2)) = cap2) |] 
+  &&  [| (n_pre <= cap1) |] 
+  &&  [| ((Zlength (l)) = n_pre) |] 
+  &&  [| (cap1 <= 100000000) |] 
+  &&  [| (list_store_Z_compact l val ) |] 
+  &&  [| ((Zlength (l2)) = cap2) |] 
+  &&  [| (cap2 >= n_pre) |] 
+  &&  [| (cap1 <= 100000000) |] 
+  &&  [| (cap2 <= 100000000) |] 
+  &&  [| (n_pre > 0) |] 
+  &&  [| (n_pre <= cap1) |]
+  &&  (store_uint_array rp_pre i l' )
+  **  (store_uint_array_rec rp_pre i cap2 l'' )
+  **  (store_uint_array ap_pre n_pre l_2 )
+  **  (store_undef_uint_array_rec ap_pre n_pre cap1 )
+.
+
+Definition mpn_add_1_partial_solve_wit_4 := mpn_add_1_partial_solve_wit_4_pure -> mpn_add_1_partial_solve_wit_4_aux.
+
+Definition mpn_add_1_partial_solve_wit_5_pure := 
+forall (b_pre: Z) (n_pre: Z) (ap_pre: Z) (rp_pre: Z) (cap2: Z) (cap1: Z) (l2: (@list Z)) (val: Z) (l: (@list Z)) (b: Z) (l'': (@list Z)) (l': (@list Z)) (val2: Z) (val1: Z) (l_2: (@list Z)) (i: Z) ,
+  [| ((unsigned_last_nbits (((Znth i l_2 0) + b )) (32)) < b) |] 
+  &&  [| (i < n_pre) |] 
+  &&  [| (0 <= i) |] 
+  &&  [| (i <= n_pre) |] 
+  &&  [| (list_store_Z_compact l_2 val ) |] 
+  &&  [| (n_pre <= cap1) |] 
+  &&  [| (list_store_Z (sublist (0) (i) (l_2)) val1 ) |] 
+  &&  [| (list_store_Z l' val2 ) |] 
+  &&  [| ((val2 + (b * (Z.pow (UINT_MOD) (i)) ) ) = (val1 + b_pre )) |] 
+  &&  [| ((Zlength (l')) = i) |] 
+  &&  [| ((Zlength (l2)) = cap2) |] 
+  &&  [| (n_pre <= cap1) |] 
+  &&  [| ((Zlength (l)) = n_pre) |] 
+  &&  [| (cap1 <= 100000000) |] 
+  &&  [| (list_store_Z_compact l val ) |] 
+  &&  [| ((Zlength (l2)) = cap2) |] 
+  &&  [| (cap2 >= n_pre) |] 
+  &&  [| (cap1 <= 100000000) |] 
+  &&  [| (cap2 <= 100000000) |] 
+  &&  [| (n_pre > 0) |] 
+  &&  [| (n_pre <= cap1) |]
+  &&  (store_uint_array ap_pre n_pre l_2 )
+  **  ((( &( "r" ) )) # UInt  |-> (unsigned_last_nbits (((Znth i l_2 0) + b )) (32)))
+  **  ((( &( "i" ) )) # Int  |-> i)
+  **  (store_undef_uint_array_rec ap_pre n_pre cap1 )
+  **  (store_uint_array rp_pre i l' )
+  **  (store_uint_array_rec rp_pre i cap2 l'' )
+  **  ((( &( "b" ) )) # UInt  |-> 1)
+  **  ((( &( "n" ) )) # Int  |-> n_pre)
+  **  ((( &( "ap" ) )) # Ptr  |-> ap_pre)
+  **  ((( &( "rp" ) )) # Ptr  |-> rp_pre)
+|--
+  [| (0 <= i) |] 
+  &&  [| (i < n_pre) |] 
+  &&  [| (n_pre <= cap2) |]
+.
+
+Definition mpn_add_1_partial_solve_wit_5_aux := 
+forall (b_pre: Z) (n_pre: Z) (ap_pre: Z) (rp_pre: Z) (cap2: Z) (cap1: Z) (l2: (@list Z)) (val: Z) (l: (@list Z)) (b: Z) (l'': (@list Z)) (l': (@list Z)) (val2: Z) (val1: Z) (l_2: (@list Z)) (i: Z) ,
+  [| ((unsigned_last_nbits (((Znth i l_2 0) + b )) (32)) < b) |] 
+  &&  [| (i < n_pre) |] 
+  &&  [| (0 <= i) |] 
+  &&  [| (i <= n_pre) |] 
+  &&  [| (list_store_Z_compact l_2 val ) |] 
+  &&  [| (n_pre <= cap1) |] 
+  &&  [| (list_store_Z (sublist (0) (i) (l_2)) val1 ) |] 
+  &&  [| (list_store_Z l' val2 ) |] 
+  &&  [| ((val2 + (b * (Z.pow (UINT_MOD) (i)) ) ) = (val1 + b_pre )) |] 
+  &&  [| ((Zlength (l')) = i) |] 
+  &&  [| ((Zlength (l2)) = cap2) |] 
+  &&  [| (n_pre <= cap1) |] 
+  &&  [| ((Zlength (l)) = n_pre) |] 
+  &&  [| (cap1 <= 100000000) |] 
+  &&  [| (list_store_Z_compact l val ) |] 
+  &&  [| ((Zlength (l2)) = cap2) |] 
+  &&  [| (cap2 >= n_pre) |] 
+  &&  [| (cap1 <= 100000000) |] 
+  &&  [| (cap2 <= 100000000) |] 
+  &&  [| (n_pre > 0) |] 
+  &&  [| (n_pre <= cap1) |]
+  &&  (store_uint_array ap_pre n_pre l_2 )
+  **  (store_undef_uint_array_rec ap_pre n_pre cap1 )
+  **  (store_uint_array rp_pre i l' )
+  **  (store_uint_array_rec rp_pre i cap2 l'' )
+|--
+  [| (0 <= i) |] 
+  &&  [| (i < n_pre) |] 
+  &&  [| (n_pre <= cap2) |] 
+  &&  [| ((unsigned_last_nbits (((Znth i l_2 0) + b )) (32)) < b) |] 
+  &&  [| (i < n_pre) |] 
+  &&  [| (0 <= i) |] 
+  &&  [| (i <= n_pre) |] 
+  &&  [| (list_store_Z_compact l_2 val ) |] 
+  &&  [| (n_pre <= cap1) |] 
+  &&  [| (list_store_Z (sublist (0) (i) (l_2)) val1 ) |] 
+  &&  [| (list_store_Z l' val2 ) |] 
+  &&  [| ((val2 + (b * (Z.pow (UINT_MOD) (i)) ) ) = (val1 + b_pre )) |] 
+  &&  [| ((Zlength (l')) = i) |] 
+  &&  [| ((Zlength (l2)) = cap2) |] 
+  &&  [| (n_pre <= cap1) |] 
+  &&  [| ((Zlength (l)) = n_pre) |] 
+  &&  [| (cap1 <= 100000000) |] 
+  &&  [| (list_store_Z_compact l val ) |] 
+  &&  [| ((Zlength (l2)) = cap2) |] 
+  &&  [| (cap2 >= n_pre) |] 
+  &&  [| (cap1 <= 100000000) |] 
+  &&  [| (cap2 <= 100000000) |] 
+  &&  [| (n_pre > 0) |] 
+  &&  [| (n_pre <= cap1) |]
+  &&  (store_uint_array rp_pre i l' )
+  **  (store_uint_array_rec rp_pre i cap2 l'' )
+  **  (store_uint_array ap_pre n_pre l_2 )
+  **  (store_undef_uint_array_rec ap_pre n_pre cap1 )
+.
+
+Definition mpn_add_1_partial_solve_wit_5 := mpn_add_1_partial_solve_wit_5_pure -> mpn_add_1_partial_solve_wit_5_aux.
+
+Definition mpn_add_1_partial_solve_wit_6 := 
+forall (b_pre: Z) (n_pre: Z) (ap_pre: Z) (rp_pre: Z) (cap2: Z) (cap1: Z) (l2: (@list Z)) (val: Z) (l: (@list Z)) (b: Z) (l'': (@list Z)) (l': (@list Z)) (val2: Z) (val1: Z) (l_2: (@list Z)) (i: Z) (a: Z) (l''': (@list Z)) ,
+  [| (l'' = (cons (a) (l'''))) |] 
+  &&  [| (0 <= i) |] 
+  &&  [| (i < n_pre) |] 
+  &&  [| (n_pre <= cap2) |] 
+  &&  [| ((unsigned_last_nbits (((Znth i l_2 0) + b )) (32)) < b) |] 
+  &&  [| (i < n_pre) |] 
+  &&  [| (0 <= i) |] 
+  &&  [| (i <= n_pre) |] 
+  &&  [| (list_store_Z_compact l_2 val ) |] 
+  &&  [| (n_pre <= cap1) |] 
+  &&  [| (list_store_Z (sublist (0) (i) (l_2)) val1 ) |] 
+  &&  [| (list_store_Z l' val2 ) |] 
+  &&  [| ((val2 + (b * (Z.pow (UINT_MOD) (i)) ) ) = (val1 + b_pre )) |] 
+  &&  [| ((Zlength (l')) = i) |] 
+  &&  [| ((Zlength (l2)) = cap2) |] 
+  &&  [| (n_pre <= cap1) |] 
+  &&  [| ((Zlength (l)) = n_pre) |] 
+  &&  [| (cap1 <= 100000000) |] 
+  &&  [| (list_store_Z_compact l val ) |] 
+  &&  [| ((Zlength (l2)) = cap2) |] 
+  &&  [| (cap2 >= n_pre) |] 
+  &&  [| (cap1 <= 100000000) |] 
+  &&  [| (cap2 <= 100000000) |] 
+  &&  [| (n_pre > 0) |] 
+  &&  [| (n_pre <= cap1) |]
+  &&  (store_uint_array_rec rp_pre (i + 1 ) cap2 l''' )
+  **  (store_uint_array rp_pre (i + 1 ) (app (l') ((cons (a) (nil)))) )
+  **  (store_uint_array ap_pre n_pre l_2 )
+  **  (store_undef_uint_array_rec ap_pre n_pre cap1 )
+|--
+  [| (l'' = (cons (a) (l'''))) |] 
+  &&  [| (0 <= i) |] 
+  &&  [| (i < n_pre) |] 
+  &&  [| (n_pre <= cap2) |] 
+  &&  [| ((unsigned_last_nbits (((Znth i l_2 0) + b )) (32)) < b) |] 
   &&  [| (i < n_pre) |] 
   &&  [| (0 <= i) |] 
   &&  [| (i <= n_pre) |] 
@@ -2280,10 +2446,74 @@ forall (b_pre: Z) (n_pre: Z) (ap_pre: Z) (rp_pre: Z) (cap2: Z) (cap1: Z) (l2: (@
   &&  [| (n_pre > 0) |] 
   &&  [| (n_pre <= cap1) |]
   &&  (((rp_pre + (i * sizeof(UINT) ) )) # UInt  |->_)
-  **  (store_uint_array_missing_i_rec rp_pre i i cap2 l'' )
+  **  (store_uint_array_missing_i_rec rp_pre i 0 (i + 1 ) (app (l') ((cons (a) (nil)))) )
+  **  (store_uint_array_rec rp_pre (i + 1 ) cap2 l''' )
   **  (store_uint_array ap_pre n_pre l_2 )
   **  (store_undef_uint_array_rec ap_pre n_pre cap1 )
-  **  (store_uint_array rp_pre i l' )
+.
+
+Definition mpn_add_1_partial_solve_wit_7 := 
+forall (b_pre: Z) (n_pre: Z) (ap_pre: Z) (rp_pre: Z) (cap2: Z) (cap1: Z) (l2: (@list Z)) (val: Z) (l: (@list Z)) (b: Z) (l'': (@list Z)) (l': (@list Z)) (val2: Z) (val1: Z) (l_2: (@list Z)) (i: Z) (a: Z) (l''': (@list Z)) ,
+  [| (l'' = (cons (a) (l'''))) |] 
+  &&  [| (0 <= i) |] 
+  &&  [| (i < n_pre) |] 
+  &&  [| (n_pre <= cap2) |] 
+  &&  [| ((unsigned_last_nbits (((Znth i l_2 0) + b )) (32)) >= b) |] 
+  &&  [| (i < n_pre) |] 
+  &&  [| (0 <= i) |] 
+  &&  [| (i <= n_pre) |] 
+  &&  [| (list_store_Z_compact l_2 val ) |] 
+  &&  [| (n_pre <= cap1) |] 
+  &&  [| (list_store_Z (sublist (0) (i) (l_2)) val1 ) |] 
+  &&  [| (list_store_Z l' val2 ) |] 
+  &&  [| ((val2 + (b * (Z.pow (UINT_MOD) (i)) ) ) = (val1 + b_pre )) |] 
+  &&  [| ((Zlength (l')) = i) |] 
+  &&  [| ((Zlength (l2)) = cap2) |] 
+  &&  [| (n_pre <= cap1) |] 
+  &&  [| ((Zlength (l)) = n_pre) |] 
+  &&  [| (cap1 <= 100000000) |] 
+  &&  [| (list_store_Z_compact l val ) |] 
+  &&  [| ((Zlength (l2)) = cap2) |] 
+  &&  [| (cap2 >= n_pre) |] 
+  &&  [| (cap1 <= 100000000) |] 
+  &&  [| (cap2 <= 100000000) |] 
+  &&  [| (n_pre > 0) |] 
+  &&  [| (n_pre <= cap1) |]
+  &&  (store_uint_array_rec rp_pre (i + 1 ) cap2 l''' )
+  **  (store_uint_array rp_pre (i + 1 ) (app (l') ((cons (a) (nil)))) )
+  **  (store_uint_array ap_pre n_pre l_2 )
+  **  (store_undef_uint_array_rec ap_pre n_pre cap1 )
+|--
+  [| (l'' = (cons (a) (l'''))) |] 
+  &&  [| (0 <= i) |] 
+  &&  [| (i < n_pre) |] 
+  &&  [| (n_pre <= cap2) |] 
+  &&  [| ((unsigned_last_nbits (((Znth i l_2 0) + b )) (32)) >= b) |] 
+  &&  [| (i < n_pre) |] 
+  &&  [| (0 <= i) |] 
+  &&  [| (i <= n_pre) |] 
+  &&  [| (list_store_Z_compact l_2 val ) |] 
+  &&  [| (n_pre <= cap1) |] 
+  &&  [| (list_store_Z (sublist (0) (i) (l_2)) val1 ) |] 
+  &&  [| (list_store_Z l' val2 ) |] 
+  &&  [| ((val2 + (b * (Z.pow (UINT_MOD) (i)) ) ) = (val1 + b_pre )) |] 
+  &&  [| ((Zlength (l')) = i) |] 
+  &&  [| ((Zlength (l2)) = cap2) |] 
+  &&  [| (n_pre <= cap1) |] 
+  &&  [| ((Zlength (l)) = n_pre) |] 
+  &&  [| (cap1 <= 100000000) |] 
+  &&  [| (list_store_Z_compact l val ) |] 
+  &&  [| ((Zlength (l2)) = cap2) |] 
+  &&  [| (cap2 >= n_pre) |] 
+  &&  [| (cap1 <= 100000000) |] 
+  &&  [| (cap2 <= 100000000) |] 
+  &&  [| (n_pre > 0) |] 
+  &&  [| (n_pre <= cap1) |]
+  &&  (((rp_pre + (i * sizeof(UINT) ) )) # UInt  |->_)
+  **  (store_uint_array_missing_i_rec rp_pre i 0 (i + 1 ) (app (l') ((cons (a) (nil)))) )
+  **  (store_uint_array_rec rp_pre (i + 1 ) cap2 l''' )
+  **  (store_uint_array ap_pre n_pre l_2 )
+  **  (store_undef_uint_array_rec ap_pre n_pre cap1 )
 .
 
 Definition mpn_add_1_which_implies_wit_1 := 
@@ -2307,6 +2537,23 @@ forall (rp_pre: Z) (cap2: Z) (l2: (@list Z)) ,
   [| ((Zlength (l2)) = cap2) |]
   &&  (store_uint_array_rec rp_pre 0 cap2 l2 )
   **  (store_uint_array rp_pre 0 nil )
+.
+
+Definition mpn_add_1_which_implies_wit_3 := 
+forall (n_pre: Z) (rp_pre: Z) (cap2: Z) (l'': (@list Z)) (l': (@list Z)) (i: Z) ,
+  [| (0 <= i) |] 
+  &&  [| (i < n_pre) |] 
+  &&  [| (n_pre <= cap2) |]
+  &&  (store_uint_array rp_pre i l' )
+  **  (store_uint_array_rec rp_pre i cap2 l'' )
+|--
+  EX (a: Z)  (l''': (@list Z)) ,
+  [| (l'' = (cons (a) (l'''))) |] 
+  &&  [| (0 <= i) |] 
+  &&  [| (i < n_pre) |] 
+  &&  [| (n_pre <= cap2) |]
+  &&  (store_uint_array_rec rp_pre (i + 1 ) cap2 l''' )
+  **  (store_uint_array rp_pre (i + 1 ) (app (l') ((cons (a) (nil)))) )
 .
 
 Module Type VC_Correct.
@@ -2390,9 +2637,14 @@ Axiom proof_of_mpn_add_1_partial_solve_wit_1 : mpn_add_1_partial_solve_wit_1.
 Axiom proof_of_mpn_add_1_partial_solve_wit_2_pure : mpn_add_1_partial_solve_wit_2_pure.
 Axiom proof_of_mpn_add_1_partial_solve_wit_2 : mpn_add_1_partial_solve_wit_2.
 Axiom proof_of_mpn_add_1_partial_solve_wit_3 : mpn_add_1_partial_solve_wit_3.
+Axiom proof_of_mpn_add_1_partial_solve_wit_4_pure : mpn_add_1_partial_solve_wit_4_pure.
 Axiom proof_of_mpn_add_1_partial_solve_wit_4 : mpn_add_1_partial_solve_wit_4.
+Axiom proof_of_mpn_add_1_partial_solve_wit_5_pure : mpn_add_1_partial_solve_wit_5_pure.
 Axiom proof_of_mpn_add_1_partial_solve_wit_5 : mpn_add_1_partial_solve_wit_5.
+Axiom proof_of_mpn_add_1_partial_solve_wit_6 : mpn_add_1_partial_solve_wit_6.
+Axiom proof_of_mpn_add_1_partial_solve_wit_7 : mpn_add_1_partial_solve_wit_7.
 Axiom proof_of_mpn_add_1_which_implies_wit_1 : mpn_add_1_which_implies_wit_1.
 Axiom proof_of_mpn_add_1_which_implies_wit_2 : mpn_add_1_which_implies_wit_2.
+Axiom proof_of_mpn_add_1_which_implies_wit_3 : mpn_add_1_which_implies_wit_3.
 
 End VC_Correct.
